rr_frontend/translation/src/body/translation/loops.rs
@@ -4,17 +4,151 @@
 // If a copy of the BSD-3-clause license was not distributed with this
 // file, You can obtain one at https://opensource.org/license/bsd-3-clause/.
 
-use log::info;
+use log::{info, trace};
 use rr_rustc_interface::hir::def_id::DefId;
-use rr_rustc_interface::middle::mir;
+use rr_rustc_interface::middle::{mir, ty};
+use rr_rustc_interface::span;
 
 use super::TX;
-use crate::attrs;
 use crate::base::*;
 use crate::environment::mir_analyses::initialization;
-use crate::spec_parsers::loop_attr_parser::{LoopAttrParser as _, VerboseLoopAttrParser};
+use crate::spec_parsers::loop_attr_parser::{LoopAttrParser as _, LoopIteratorInfo, VerboseLoopAttrParser};
+use crate::{attrs, search, types};
 
 impl<'a, 'def: 'a, 'tcx: 'def> TX<'a, 'def, 'tcx> {
+    fn check_operand_call_dest(&self, op: &mir::Operand<'tcx>) -> Option<DefId> {
+        let ty = self.get_type_of_operand(op);
+        match ty.kind() {
+            ty::TyKind::FnDef(did, _) => Some(*did),
+            _ => None,
+        }
+    }
+
+    fn find_origin_of_mut_bor(&self, var: mir::Local, bb: mir::BasicBlock) -> mir::Local {
+        let proc = self.proc;
+        let mir = proc.get_mir();
+        let bb_data = &mir.basic_blocks[bb];
+        let stmts = &bb_data.statements;
+
+        let mut current_var = var;
+        for stmt in stmts.iter().rev() {
+            if let mir::StatementKind::Assign(assign) = &stmt.kind {
+                let plc = &assign.0;
+                let val = &assign.1;
+
+                if plc.local != current_var {
+                    continue;
+                }
+
+                assert!(plc.projection.is_empty());
+                // find the RHS
+                let mir::Rvalue::Ref(_, _, plc) = val else {
+                    unimplemented!();
+                };
+
+                // the place might directly refer to the destination variable or be a Deref due to reborrow
+                if plc.projection.is_empty() {
+                    current_var = plc.local;
+                } else if plc.projection.len() == 1 {
+                    current_var = plc.local;
+
+                    assert!(matches!(plc.projection[0], mir::ProjectionElem::Deref));
+                } else {
+                    unimplemented!();
+                }
+            }
+        }
+
+        current_var
+    }
+
+    fn check_for_iter_next(
+        &self,
+        bb: mir::BasicBlock,
+    ) -> Result<Option<LoopIteratorInfo<'def>>, TranslationError<'tcx>> {
+        let proc = self.proc;
+        let mir = proc.get_mir();
+        let bb_data = &mir.basic_blocks[bb];
+        let term = bb_data.terminator();
+
+        let mir::TerminatorKind::Call { func, args, .. } = &term.kind else {
+            return Ok(None);
+        };
+
+        let fn_ty = self.get_type_of_operand(func);
+        let call_dest = self.check_operand_call_dest(func).unwrap();
+
+        let iterator_did = search::try_resolve_did(self.env.tcx(), &["core", "iter", "Iterator"]).unwrap();
+        let iterator_items: &ty::AssocItems = self.env.tcx().associated_items(iterator_did);
+        let next_symbol = span::Symbol::intern("next");
+        let next_ident = span::Ident::with_dummy_span(next_symbol);
+        let next_item = iterator_items
+            .find_by_ident_and_kind(self.env.tcx(), next_ident, ty::AssocTag::Fn, iterator_did)
+            .unwrap();
+
+        if next_item.def_id != call_dest {
+            return Ok(None);
+        }
+
+        // now trace the argument back to before the mutable borrow
+        let next_ref_arg = &args[0].node;
+        let mir::Operand::Move(plc) = next_ref_arg else {
+            return Ok(None);
+        };
+        assert!(plc.projection.is_empty());
+        let next_ref_local = plc.local;
+
+        let iter_variable = self.find_origin_of_mut_bor(next_ref_local, bb);
+
+        trace!("check_for_iter_next: found iterator variable {iter_variable:?}");
+
+        // so: I'm calling next here.
+        // I can definitely resolve that method call.
+        // I will go either into the UserDefined or the Param path.
+        // I want to find the instantiation of the Iterator trait, right?
+        // Then I will be able to refer to the attribute term of that.
+
+        let ty::TyKind::FnDef(_, params) = fn_ty.kind() else {
+            return Err(TranslationError::UnknownError("not a FnDef type".to_owned()));
+        };
+
+        // exploiting that Iterator has the same args as Iterator::next
+        let mut scope = self.ty_translator.scope.borrow_mut();
+        let mut state = types::STInner::InFunction(&mut scope);
+        let trait_spec_term = self.trait_registry.resolve_trait_requirement_in_state(
+            &mut state,
+            iterator_did,
+            params,
+            ty::Binder::dummy(()),
+            &[],
+            radium::TyParamOrigin::Direct,
+            &[],
+        )?;
+        let trait_spec_term =
+            self.trait_registry.translate_trait_req_inst_in_state(&mut state, trait_spec_term)?;
+        trace!("trait_spec_term={trait_spec_term:?}");
+
+        Ok(Some(LoopIteratorInfo {
+            iterator_variable: iter_variable,
+            binder_name: format!("_iter_{}", iter_variable.index()),
+            iter_spec: trait_spec_term,
+        }))
+    }
+
+    fn check_is_for_loop(
+        &self,
+        loop_head: mir::BasicBlock,
+    ) -> Result<Option<LoopIteratorInfo<'def>>, TranslationError<'tcx>> {
+        let proc = self.proc;
+        let succs = proc.successors(loop_head);
+
+        if succs.len() == 1 {
+            return self.check_for_iter_next(succs[0]);
+        }
+
+        Ok(None)
+    }
+
     /// Parse the attributes on spec closure `did` as loop annotations and add it as an invariant
     /// to the generated code.
     pub(crate) fn parse_attributes_on_loop_spec_closure(
@@ -22,22 +156,29 @@ impl<'a, 'def: 'a, 'tcx: 'def> TX<'a, 'def, 'tcx> {
         loop_head: mir::BasicBlock,
         did: Option<DefId>,
     ) -> Result<radium::LoopSpec, TranslationError<'tcx>> {
-        // determine invariant on initialization:
-        // - we need this both for the refinement invariant (though this could be removed if we make uninit
-        //   generic over the refinement)
-        // - in order to establish the initialization invariant in each loop iteration, since we don't have
-        //   proper subtyping for uninit => maybe we could fix this too by making uninit variant in the
-        //   refinement type? then we could have proper subtyping lemmas.
-        //  + to bring it to the right refinement type initially, maybe have some automation /
-        //  annotation
-        // TODO: consider changing it like that.
-        //
         // Note that StorageDead will not help us for determining initialization/ making it invariant, since
         // it only applies to full stack slots, not individual paths. one thing that makes it more
         // complicated in the frontend: initialization may in practice also be path-dependent.
         //  - this does not cause issues with posing a too strong loop invariant,
         //  - but this poses an issue for annotations
         //
+
+        // Plan:
+        // - pass the iter variable to the loop parser
+        // - if we want to use the Next relation, we need to figure out the appropriate trait info
+        // to use here.
+        //   maybe we can do that by getting some info from the next call?
+        //   But having the attrs available in that place of the function seems a bit difficult.
+        //   Maybe if I'm giving names to all parameters of the proof and introduce them
+        //   accordingly.
+        //   let's try this later.
+        //   but for now, let's just give a special name to the iterator state and then see later
+        //   for more advanced stuff.
+        //
+        // One difficulty: when I prove invariant conditions later, I won't have the SL context
+        // available. Need to be a bit careful.
+        //
+        let iterator_info = self.check_is_for_loop(loop_head)?;
 
         let init_result = initialization::compute_definitely_initialized(
             self.proc.get_id(),
@@ -47,18 +188,29 @@ impl<'a, 'def: 'a, 'tcx: 'def> TX<'a, 'def, 'tcx> {
         let init_places = init_result.get_before_block(loop_head);
 
         // get locals
-        let mut locals_with_initialization: Vec<(String, radium::LocalKind, bool, radium::Type<'def>)> =
-            Vec::new();
+        let mut locals_with_initialization: Vec<(
+            mir::Local,
+            String,
+            radium::LocalKind,
+            bool,
+            radium::Type<'def>,
+        )> = Vec::new();
 
         for (local, kind, name, ty) in &self.fn_locals {
             let place = mir::Place::from(*local);
             let initialized = init_places.contains(place);
 
-            locals_with_initialization.push((name.to_owned(), kind.to_owned(), initialized, ty.to_owned()));
+            locals_with_initialization.push((
+                *local,
+                name.to_owned(),
+                kind.to_owned(),
+                initialized,
+                ty.to_owned(),
+            ));
         }
 
         let scope = self.ty_translator.scope.borrow();
-        let mut parser = VerboseLoopAttrParser::new(locals_with_initialization, &*scope);
+        let mut parser = VerboseLoopAttrParser::new(locals_with_initialization, &*scope, iterator_info);
 
         if let Some(did) = did {
             let attrs = self.env.get_attributes(did);
