rr_frontend/translation/src/environment/procedure.rs
@@ -72,4 +72,10 @@ impl<'tcx> Procedure<'tcx> {
     pub(crate) fn predecessors(&self, bbi: mir::BasicBlock) -> &[mir::BasicBlock] {
         self.real_edges.predecessors(bbi)
     }
+
+    /// Get the successors of a basic block.
+    #[must_use]
+    pub(crate) fn successors(&self, bbi: mir::BasicBlock) -> &[mir::BasicBlock] {
+        self.real_edges.successors(bbi)
+    }
 }
