stdlib/iterator/extra_specs.v
@@ -2,7 +2,7 @@ Section trans.
   
   Fixpoint IteratorNextFusedTrans {Self_rt Item_rt : RT} 
     (attrs : traits_iterator_Iterator_spec_attrs Self_rt Item_rt)
-    (s1 : Self_rt) (els : list (Item_rt)) (s2 : Self_rt) : iProp Σ
+    (s1 : RT_xt Self_rt) (els : list (RT_xt Item_rt)) (s2 : RT_xt Self_rt) : iProp Σ
     :=
     match els with
     | [] => ⌜s1 = s2⌝
@@ -12,23 +12,44 @@ Section trans.
         IteratorNextFusedTrans attrs s1' els s2
     end.
 
-  (* Steps for loops with iterators:
-     - set a variable with the initial state in the context
-       (we need a special identifier for that, I guess?)
-     - add invariant using IteratorNextFusedTrans from the initial state to the current iterator state.
-       
+  Lemma iterator_next_fused_trans_app {Self_rt Item_rt : RT} (A : traits_iterator_Iterator_spec_attrs Self_rt Item_rt) s1 hist s2 x :
+    IteratorNextFusedTrans A s1 (hist ++ [x]) s2 ⊣⊢ (∃ s2', IteratorNextFusedTrans A s1 hist s2' ∗ A.(traits_iterator_Iterator_Next) s2' (Some x) s2).
+  Proof.
+    iInduction hist as [ | y hist] "IH" forall (s1 s2); simpl.
+    - iSplit.
+      + iIntros "(%s1' & ? & <-)". by iFrame.
+      + iIntros "(%s2' & -> & ?)". by iFrame.
+    - iSplit.
+      + iIntros "(%s1' & Ha & Hb)".
+        iPoseProof ("IH" with "Hb") as "(%s2' & Hb & Hc)".
+        iFrame.
+      + iIntros "(%s2' & (%s1' & ? & ?) & ?)".
+        iFrame. iApply "IH". iFrame.
+  Qed.
 
-     Frontend: 
-     - identify that we have a for loop
-     - find the iterator variable
-     - add it to the set of variables we need an invariant on
-     - etc. 
+  Lemma simplify_goal_iterator_next_fused_trans_app {Self_rt Item_rt : RT} (A : traits_iterator_Iterator_spec_attrs Self_rt Item_rt) s1 hist s2 s1' hist' `{!CheckOwnInContext (IteratorNextFusedTrans A s1 hist' s1')} T :
+    (∃ x, 
+      ⌜hist = hist' ++ [x]⌝ ∗
+      IteratorNextFusedTrans A s1 hist' s1' ∗
+      A.(traits_iterator_Iterator_Next) s1' (Some x) s2) ∗ T ⊢ simplify_goal (IteratorNextFusedTrans A s1 hist s2) T.
+  Proof.
+    rewrite /simplify_goal. 
+    iIntros "((%x & -> & Ha & Hb) & $)".
+    rewrite iterator_next_fused_trans_app.
+    iFrame.
+  Qed.
+  Definition simplify_goal_iterator_next_fused_trans_app_inst := [instance @simplify_goal_iterator_next_fused_trans_app with 50%N].
+  Global Existing Instance simplify_goal_iterator_next_fused_trans_app_inst.
 
-   *)
-
-  (* TODO: we might need some Lithium instances to automate the SL reasoning here. 
-     Is Next opaque for us? I guess it should unfold. Let's just see how it works.
-  *)
+  Lemma simplify_goal_iterator_next_fused_trans_nil {Self_rt Item_rt : RT} (A : traits_iterator_Iterator_spec_attrs Self_rt Item_rt) s1 hist T :
+    (⌜hist = []⌝) ∗ T ⊢ simplify_goal (IteratorNextFusedTrans A s1 hist s1) T.
+  Proof.
+    rewrite /simplify_goal.
+    iIntros "(-> & $)".
+    eauto.
+  Qed.
+  Definition simplify_goal_iterator_next_fused_trans_nil_inst := [instance @simplify_goal_iterator_next_fused_trans_nil with 10%N].
+  Global Existing Instance simplify_goal_iterator_next_fused_trans_nil_inst.
 
 
 End trans.
