case_studies/extra_proofs/tests/loops.v
@@ -1,0 +1,71 @@
+From refinedrust Require Import typing.
+
+(* TODO upstream *)
+
+Definition sum_list_Z_with {A} (f : A → Z) : list A → Z :=
+  fix go l :=
+  match l with
+  | [] => 0
+  | x :: l => f x + go l
+  end.
+Notation sum_list_Z := (sum_list_Z_with id).
+
+
+(** ** Properties of the [sum_list_Z_with] function *)
+Section sum_list.
+  Context {A : Type}.
+  Implicit Types x y z : A.
+  Implicit Types l k : list A.
+  Lemma sum_list_Z_with_app (f : A → Z) l k :
+    sum_list_Z_with f (l ++ k) = sum_list_Z_with f l + sum_list_Z_with f k.
+  Proof. induction l; simpl; lia. Qed.
+  Lemma sum_list_Z_with_reverse (f : A → Z) l :
+    sum_list_Z_with f (reverse l) = sum_list_Z_with f l.
+  Proof.
+    induction l; simpl; rewrite ?reverse_cons ?sum_list_Z_with_app; simpl; lia.
+  Qed.
+  Lemma sum_list_Z_fmap_same n l f :
+    Forall (λ x, f x = n) l →
+    sum_list_Z (f <$> l) = length l * n.
+  Proof. induction 1; csimpl; lia. Qed.
+  Lemma sum_list_Z_fmap_const l n :
+    sum_list_Z ((λ _, n) <$> l) = length l * n.
+  Proof. by apply sum_list_Z_fmap_same, Forall_true. Qed.
+End sum_list.
+
+Global Hint Rewrite -> @sum_list_Z_with_app : lithium_rewrite.
+
+Lemma seqZ_pos_seq start count :
+  0 ≤ start →
+  seqZ start count = Z.of_nat <$> seq (Z.to_nat start) (Z.to_nat count).
+Proof.
+  intros Hge.
+  set (start' := Z.to_nat start).
+  assert (start = Z.of_nat start') as Heq by lia.
+  rewrite Heq in Hge.
+  rewrite Heq.
+  generalize start'.
+  clear. intros start.
+  unfold seqZ.
+  generalize (Z.to_nat count) as count'. 
+  clear. intros count.
+  unfold fmap.
+  (*induction count as [ | ? IH] in start |-*; simpl; try solve_goal.*)
+  (*f_equiv; first lia.*)
+  (*rewrite -IH.*)
+  (*solve_goal.*)
+Admitted.
+Global Hint Rewrite -> seqZ_pos_seq using lia : lithium_rewrite.
+
+(* Idea more generally: split at 0 *)
+
+Lemma sum_list_Z_of_nat xs :
+  sum_list_Z (Z.of_nat <$> xs) = sum_list xs.
+Proof.
+Admitted.
+Global Hint Rewrite -> sum_list_Z_of_nat : lithium_rewrite.
+
+Global Hint Rewrite -> Z2Nat.inj_0 : lithium_rewrite.
+Global Hint Rewrite -> Z.sub_0_r Z.add_0_r Z.sub_0_l Z.add_0_l : lithium_rewrite.
+
+
