case_studies/tests/output/tests/proofs/proof_loops_loop4_myrange.v
@@ -1,0 +1,29 @@
+From caesium Require Import lang notation.
+From refinedrust Require Import typing shims.
+From refinedrust.examples.tests.generated Require Import generated_code_tests generated_specs_tests generated_template_loops_loop4_myrange.
+
+Set Default Proof Using "Type".
+
+From iris.proofmode Require Import coq_tactics reduction string_ident.
+
+
+Section proof.
+Context `{RRGS : !refinedrustGS Σ}.
+
+Lemma loops_loop4_myrange_proof (π : thread_id) :
+  loops_loop4_myrange_lemma π.
+Proof.
+  loops_loop4_myrange_prelude.
+
+  rep liRStep; liShow.
+
+  all: print_remaining_goal.
+  Unshelve. all: sidecond_solver.
+  Unshelve. all: sidecond_hammer.
+
+  1-3: admit.
+
+  Unshelve. all: print_remaining_sidecond.
+(*Qed.*)
+Admitted.
+End proof.
