case_studies/tests/output/tests/proofs/proof_loops_loop4_myrange_2.v
@@ -1,0 +1,48 @@
+From caesium Require Import lang notation.
+From refinedrust Require Import typing shims.
+From refinedrust.examples.tests.generated Require Import generated_code_tests generated_specs_tests generated_template_loops_loop4_myrange_2.
+
+Set Default Proof Using "Type".
+
+Section proof.
+Context `{RRGS : !refinedrustGS Σ}.
+
+
+Program Instance learn_from_hyp_range_it s1 hist s2 :
+  LearnFromHyp (IteratorNextFusedTrans loops_MyRangeasstd_iter_Iterator_spec_attrs s1 hist s2) :=
+  {| learn_from_hyp_Q := ⌜s1.2 = s2.2 ∧ s1.1 ≤ s2.1 ∧ (* s2.1 ≤ s2.2 ∧ *) hist = seqZ s1.1 (s2.1 - s1.1)⌝%I |}.
+Next Obligation.
+  iIntros (?????) "Hx".
+  iModIntro.
+  iInduction hist as [ | x hist] "IH" forall (s1 s2); simpl.
+  { iDestruct "Hx" as "%". subst. iPureIntro.
+    rewrite Z.sub_diag. done. }
+  iDestruct "Hx" as "(%s1' & %Ha & Hx)".
+  iPoseProof ("IH" with "Hx") as "($ & %Hb)".
+  iPureIntro.
+  destruct Ha as (? & _ & <- & ? & ?). destruct Hb as (? & ? & ->).
+  destruct s1, s2, s1'; simpl in *.
+  subst. split_and!; try solve_goal.
+  assert (1 ≤ r1 - r) as Hge by lia.
+  rewrite Z.sub_add_distr.
+  assert ((r1 - 1 -r)%Z = ((r1 - r) - 1)%Z) as -> by lia.
+  move: Hge. generalize (r1 - r) as x.
+Admitted.
+
+Lemma loops_loop4_myrange_2_proof (π : thread_id) :
+  loops_loop4_myrange_2_lemma π.
+Proof.
+  loops_loop4_myrange_2_prelude.
+
+  rep liRStep; liShow.
+
+  all: print_remaining_goal.
+  Unshelve. all: sidecond_solver.
+  Unshelve. all: sidecond_hammer.
+  { simpl.
+    admit. }
+  { admit. }
+  Unshelve. all: print_remaining_sidecond.
+(*Qed.*)
+Admitted.
+End proof.
